src/opt/Merge.v
@@ -26,20 +26,20 @@ Require Import Semantics.
 Set Implicit Arguments.
 
 Lemma assign_sim_thread:
-  forall r1 r2
+  forall v1 r2
     rs_src rs_tgt lc_src lc_tgt mem_k_src mem_k_tgt
-    (RS: rs_src = RegFun.add r2 (rs_tgt r1) rs_tgt)
+    (RS: rs_src = RegFun.add r2 (RegFile.eval_value rs_tgt v1) rs_tgt)
     (LOCAL: sim_local lc_src lc_tgt),
     sim_thread
       (sim_terminal eq)
       (State.mk rs_src [Stmt.instr Instr.skip]) lc_src mem_k_src
-      (State.mk rs_tgt [Stmt.instr (Instr.assign r2 (Instr.expr_val (Value.reg r1)))]) lc_tgt mem_k_tgt.
+      (State.mk rs_tgt [Stmt.instr (Instr.assign r2 (Instr.expr_val v1))]) lc_tgt mem_k_tgt.
 Proof.
   pcofix CIH. i. pfold. ii. splits.
   { i. inv TERMINAL_TGT. }
   { i. eapply sim_local_future; try apply MEMORY; eauto. apply LOCAL. }
   { i. eexists _, _, _. splits; eauto.
-    inv LOCAL. apply MemInv.sem_bot_inv in PROMISES. rewrite PROMISES. auto.
+    eapply sim_local_memory_bot; eauto.
   }
   ii. inv STEP_TGT; inv STEP; try (inv STATE; inv INSTR); ss.
   - (* promise *)
@@ -72,7 +72,7 @@ Proof.
   { i. inv TERMINAL_TGT. }
   { i. eapply sim_local_future; try apply MEMORY; eauto. apply LOCAL. }
   { i. eexists _, _, _. splits; eauto.
-    inv LOCAL. apply MemInv.sem_bot_inv in PROMISES. rewrite PROMISES. auto.
+    eapply sim_local_memory_bot; eauto.
   }
   ii. inv STEP_TGT; inv STEP; try (inv STATE; inv INSTR); ss.
   - (* promise *)
@@ -94,10 +94,226 @@ Proof.
     + eauto.
     + eauto.
     + left. eapply paco7_mon.
-      * apply assign_sim_thread; eauto.
-        unfold RegFun.add, RegFun.find. repeat condtac; auto. congr.
+      * apply assign_sim_thread; eauto. s. rewrite RegFun.add_spec_eq. auto.
       * i. inv PR.
 Qed.
+
+Lemma merge_store_load_sim_stmts
+      l
+      v1 o1
+      r2 o2
+      (O2: Ordering.le o2 Ordering.acqrel):
+  sim_stmts eq
+            [Stmt.instr (Instr.store l v1 o1); Stmt.instr (Instr.load r2 l o2); Stmt.instr Instr.skip]
+            [Stmt.instr (Instr.store l v1 o1); Stmt.instr (Instr.assign r2 v1)]
+            eq.
+Proof.
+  pcofix CIH. ii. subst. pfold. ii. splits.
+  { i. inv TERMINAL_TGT. }
+  { i. eapply sim_local_future; try apply MEMORY; eauto. apply LOCAL. }
+  { i. eexists _, _, _. splits; eauto.
+    eapply sim_local_memory_bot; eauto.
+  }
+  ii. inv STEP_TGT; inv STEP; try (inv STATE; inv INSTR); ss.
+  - (* promise *)
+    exploit sim_local_promise; eauto. i. des.
+    eexists _, _, _, _, _, _, _. splits; eauto.
+    econs 1; eauto. econs; eauto. eauto.
+  - (* store *)
+    exploit merge_write_read1; eauto. i. des.
+    exploit sim_local_write; try apply STEP1; eauto. i. des.
+    exploit sim_local_read; try apply STEP2; eauto.
+    { eapply Local.write_step_future; eauto. }
+    { eapply Local.write_step_future; eauto. }
+    i. des.
+    eexists _, _, _, _, _, _, _. splits.
+    + econs 2; [|econs 1]. econs.
+      * econs 2. econs 3; eauto. econs. econs.
+      * eauto.
+    + econs 2. econs 2; eauto. econs. econs.
+    + eauto.
+    + eauto.
+    + left. eapply paco7_mon.
+      * apply assign_sim_thread; auto.
+      * i. inv PR.
+Qed.
+
+Lemma merge_store_store_sim_stmts
+      l
+      v1 o1
+      v2 o2
+      o
+      (O1: Ordering.le o1 o)
+      (O2: Ordering.le o2 o):
+  sim_stmts eq
+            [Stmt.instr (Instr.store l v1 o1); Stmt.instr (Instr.store l v2 o2)]
+            [Stmt.instr (Instr.store l v2 o)]
+            eq.
+Proof.
+  pcofix CIH. ii. subst. pfold. ii. splits.
+  { i. inv TERMINAL_TGT. }
+  { i. eapply sim_local_future; try apply MEMORY; eauto. apply LOCAL. }
+  { i. eexists _, _, _. splits; eauto.
+    eapply sim_local_memory_bot; eauto.
+  }
+  ii. inv STEP_TGT; inv STEP; try (inv STATE; inv INSTR); ss.
+  - (* promise *)
+    exploit sim_local_promise; eauto. i. des.
+    eexists _, _, _, _, _, _, _. splits; eauto.
+    econs 1; eauto. econs; eauto. eauto.
+  - (* store *)
+    exploit merge_write_write; try apply LOCAL0; [apply O1|apply O2| | |]; eauto. i. des.
+    exploit sim_local_write; try apply STEP1; eauto. i. des.
+    exploit sim_local_write; try apply STEP2; eauto.
+    { eapply Local.write_step_future; eauto. }
+    { eapply Local.write_step_future; eauto. }
+    { eapply Local.write_step_future; eauto. }
+    { eapply Local.write_step_future; eauto. }
+    i. des.
+    eexists _, _, _, _, _, _, _. splits.
+    + econs 2; [|econs 1]. econs.
+      * econs 2. econs 3; eauto. econs. econs.
+      * eauto.
+    + econs 2. econs 3; eauto. econs. econs.
+    + eauto.
+    + etrans; eauto.
+    + left. eapply paco7_mon.
+      * apply sim_stmts_nil; eauto.
+      * ii. inv PR.
+Grab Existential Variables.
+  { apply Time.elt. }
+  { apply Capability.elt. }
+Qed.
+
+Lemma merge_store_update_sim_stmts
+      l
+      v1 o1
+      r2 or2 ow2
+      o
+      (O1: Ordering.le o1 o)
+      (OW2: Ordering.le ow2 o)
+      (OR2: Ordering.le or2 Ordering.acqrel):
+  sim_stmts eq
+            [Stmt.instr (Instr.store l v1 o1); Stmt.instr (Instr.update r2 l (Instr.fetch_add (Value.const 0)) or2 ow2); Stmt.instr Instr.skip]
+            [Stmt.instr (Instr.store l v1 o); Stmt.instr (Instr.assign r2 v1)]
+            eq.
+Proof.
+  pcofix CIH. ii. subst. pfold. ii. splits.
+  { i. inv TERMINAL_TGT. }
+  { i. eapply sim_local_future; try apply MEMORY; eauto. apply LOCAL. }
+  { i. eexists _, _, _. splits; eauto.
+    eapply sim_local_memory_bot; eauto.
+  }
+  ii. inv STEP_TGT; inv STEP; try (inv STATE; inv INSTR); ss.
+  - (* promise *)
+    exploit sim_local_promise; eauto. i. des.
+    eexists _, _, _, _, _, _, _. splits; eauto.
+    econs 1; eauto. econs; eauto. eauto.
+  - (* store *)
+    exploit merge_write_write; try apply LOCAL0; [apply O1|apply OW2| | |]; eauto. i. des.
+    exploit merge_write_read1; try apply STEP1; eauto. i. des.
+    exploit Local.write_step_future; eauto. i. des.
+    exploit sim_local_write; try apply STEP0; eauto. i. des.
+    exploit Local.write_step_future; eauto. i. des.
+    exploit sim_local_read; try apply STEP3; eauto. i. des.
+    exploit sim_local_write; try apply STEP2; eauto.
+    { eapply Local.read_step_future; eauto. }
+    { eapply Local.read_step_future; eauto. }
+    i. des.
+    eexists _, _, _, _, _, _, _. splits.
+    + econs 2; [|econs 1]. econs.
+      * econs 2. econs 3; eauto. econs. econs.
+      * eauto.
+    + econs 2. econs 4; eauto.
+      * econs. econs. econs.
+      * rewrite Const.add_0_r. rewrite Capability.le_join_r; eauto. refl.
+    + eauto.
+    + etrans; eauto.
+    + left. eapply paco7_mon.
+      * apply assign_sim_thread; eauto. ss. rewrite Const.add_0_r. auto.
+      * ii. inv PR.
+Grab Existential Variables.
+  { apply Time.elt. }
+Qed.
+
+(* TODO: check the condition `OR1` *)
+Lemma merge_update_load_sim_stmts
+      l
+      r1 v1 or1 ow1
+      r2 o2
+      (OR1: Ordering.le Ordering.relaxed or1)
+      (O2: Ordering.le o2 Ordering.relaxed):
+  sim_stmts eq
+            [Stmt.instr (Instr.update r1 l (Instr.fetch_add v1) or1 ow1); Stmt.instr (Instr.load r2 l o2); Stmt.instr Instr.skip]
+            [Stmt.instr (Instr.update r1 l (Instr.fetch_add v1) or1 ow1); Stmt.instr (Instr.assign r2 r1)]
+            eq.
+Proof.
+  pcofix CIH. ii. subst. pfold. ii. splits.
+  { i. inv TERMINAL_TGT. }
+  { i. eapply sim_local_future; try apply MEMORY; eauto. apply LOCAL. }
+  { i. eexists _, _, _. splits; eauto.
+    eapply sim_local_memory_bot; eauto.
+  }
+  ii. inv STEP_TGT; inv STEP; try (inv STATE; inv INSTR); ss.
+  - (* promise *)
+    exploit sim_local_promise; eauto. i. des.
+    eexists _, _, _, _, _, _, _. splits; eauto.
+    econs 1; eauto. econs; eauto. eauto.
+  - (* update *)
+    exploit Local.read_step_future; eauto. i. des.
+    exploit merge_write_read2; try apply LOCAL2; eauto.
+    { inv LOCAL1. apply COMMIT. }
+    { inv LOCAL1. apply COMMIT. auto. }
+    i. des.
+    exploit sim_local_read; try apply LOCAL1; eauto. i. des.
+    exploit Local.read_step_future; eauto. i. des.
+    exploit sim_local_write; try apply STEP1; eauto. i. des.
+    exploit sim_local_read; try apply STEP2; eauto.
+    { eapply Local.write_step_future; eauto. }
+    { eapply Local.write_step_future; eauto. }
+    i. des.
+    eexists _, _, _, _, _, _, _. splits.
+    + econs 2; [|econs 1]. econs.
+      * econs 2. econs 4; eauto. econs. econs. eauto.
+      * eauto.
+    + econs 2. econs 2; eauto. econs. econs.
+    + eauto.
+    + eauto.
+    + left. eapply paco7_mon.
+      * apply assign_sim_thread; auto. s. rewrite RegFun.add_spec_eq. inv RMW. auto.
+      * i. inv PR.
+Qed.
+
+Lemma merge_update_update_sim_stmts
+      l
+      r1 v1 or1 ow1
+      r2 or2 ow2
+      or ow
+      (OR1_RLX: Ordering.le Ordering.relaxed or1)
+      (OR2_RLX: Ordering.le or2 Ordering.relaxed)
+      (OW1: Ordering.le ow1 ow)
+      (OW2: Ordering.le ow2 ow)
+      (OR1: Ordering.le or1 or)
+      (OR2: Ordering.le or2 or):
+  sim_stmts eq
+            [Stmt.instr (Instr.update r1 l (Instr.fetch_add v1) or1 ow1); Stmt.instr (Instr.update r2 l (Instr.fetch_add 0) or2 ow2); Stmt.instr Instr.skip]
+            [Stmt.instr (Instr.update r1 l (Instr.fetch_add v1) or ow); Stmt.instr (Instr.assign r2 r1)]
+            eq.
+Proof.
+  pcofix CIH. ii. subst. pfold. ii. splits.
+  { i. inv TERMINAL_TGT. }
+  { i. eapply sim_local_future; try apply MEMORY; eauto. apply LOCAL. }
+  { i. eexists _, _, _. splits; eauto.
+    eapply sim_local_memory_bot; eauto.
+  }
+  ii. inv STEP_TGT; inv STEP; try (inv STATE; inv INSTR); ss.
+  - (* promise *)
+    exploit sim_local_promise; eauto. i. des.
+    eexists _, _, _, _, _, _, _. splits; eauto.
+    econs 1; eauto. econs; eauto. eauto.
+  - (* update *)
+    admit.
+Admitted.
 
 Lemma merge_fence_fence_sim_stmts
       ordr1 ordw1
@@ -116,7 +332,7 @@ Proof.
   { i. inv TERMINAL_TGT. }
   { i. eapply sim_local_future; try apply MEMORY; eauto. apply LOCAL. }
   { i. eexists _, _, _. splits; eauto.
-    inv LOCAL. apply MemInv.sem_bot_inv in PROMISES. rewrite PROMISES. auto.
+    eapply sim_local_memory_bot; eauto.
   }
   ii. inv STEP_TGT; inv STEP; try (inv STATE; inv INSTR); ss.
   - (* promise *)
