src/opt/MergeMemory.v
@@ -1,0 +1,52 @@
+Require Import Basics.
+Require Import Bool.
+Require Import List.
+
+Require Import sflib.
+Require Import paco.
+Require Import respectful5.
+
+Require Import Basic.
+Require Import Event.
+Require Import Language.
+Require Import Time.
+Require Import Memory.
+Require Import Commit.
+Require Import Thread.
+
+Require Import Configuration.
+Require Import Simulation.
+Require Import Compatibility.
+Require Import MemInv.
+
+Require Import Syntax.
+Require Import Semantics.
+
+Set Implicit Arguments.
+
+
+Lemma fulfill_promise_fulfill_fulfill
+      promises1 loc ts1 ts2 ts3 msg1 msg2 promises4
+      mem1
+      (LE: Memory.le promises1 mem1)
+      (FULFILL: Memory.fulfill promises1 loc ts1 ts3 msg2 promises4):
+  exists promises2 mem2 promises3,
+    <<SPLIT: Memory.promise promises1 mem1 loc ts1 ts2 msg1 promises2 mem2 Memory.promise_kind_split>> /\
+    <<FULFILL1: Memory.fulfill promises2 loc ts1 ts2 msg1 promises3>> /\
+    <<FULFILL2: Memory.fulfill promises3 loc ts2 ts3 msg2 promises4>>.
+Proof.
+Admitted.
+
+Lemma promise_fulfill_promise_fulfill_promise_fulfill
+      promises1 loc ts1 ts2 ts3 msg1 msg2 promises4 promises5
+      mem1 mem4
+      (LE: Memory.le promises1 mem1)
+      (PROMISE: Memory.promise promises1 mem1 loc ts1 ts3 msg2 promises4 mem4 Memory.promise_kind_add)
+      (FULFILL: Memory.fulfill promises4 loc ts1 ts3 msg2 promises5):
+  exists promises2 mem2 promises3 promises4 mem4,
+    <<PROMISE1: Memory.promise promises1 mem1 loc ts1 ts2 msg1 promises2 mem2 Memory.promise_kind_add>> /\
+    <<FULFILL1: Memory.fulfill promises2 loc ts1 ts2 msg1 promises3>> /\
+    <<PROMISE2: Memory.promise promises3 mem2 loc ts2 ts3 msg2 promises4 mem4 Memory.promise_kind_add>> /\
+    <<FULFILL2: Memory.fulfill promises4 loc ts2 ts3 msg2 promises5>>.
+Proof.
+Admitted.
